src/IMP.v
@@ -1,0 +1,159 @@
+Add LoadPath "./" as Monads .
+(*Require Import Monads.FunctorApplicativeMonad.*)
+Require Import Monads.ExnMonad.
+(*Require Import Monads.ExnTransformer.*)
+Require Import NPeano Arith Bool String List.
+
+Definition state:= string -> nat.
+Definition eqb_string (x y : string) : bool :=
+  if string_dec x y then true else false.
+
+Definition state_update  (m : state )
+                    (x : string) (v : nat) :=
+  fun x' => if eqb_string x x' then v else m x'.
+  
+Definition newarray (n : nat) : state :=
+  (fun _ => n).
+
+Notation "'_' '!->' v" := (newarray v)
+  (at level 100, right associativity).
+
+Definition empty_st := (_ !-> 0).
+
+
+Inductive exp : Type :=
+  | ANum (n : nat)
+  | AId (x : string)             
+  | APlus (a1 a2 : exp)
+  | ADiv (a1 a2: exp)
+  | EqExp (a1 a2: exp).
+
+Coercion AId : string >-> exp.
+Coercion ANum : nat >-> exp.
+
+Declare Custom Entry com.
+Declare Scope com_scope.
+Notation "<{ e }>" := e (at level 0, e custom com at level 99) : com_scope.
+Notation "( x )" := x (in custom com, x at level 99) : com_scope.
+Notation "x" := x (in custom com at level 0, x constr at level 0) : com_scope.
+Notation "f x .. y" := (.. (f x) .. y)
+                  (in custom com at level 0, only parsing,
+                  f constr at level 0, x constr at level 9,
+                  y constr at level 9) : com_scope.
+Notation "x + y" := (APlus x y) (in custom com at level 50, left associativity).
+Notation "x / y" := (ADiv x y) (in custom com at level 50, left associativity).
+Notation "x == y" := (EqExp x y) (in custom com at level 50, left associativity).
+Open Scope com_scope.
+
+Definition X:string:="x"%string.
+Definition Y:string:="y"%string.
+Definition Z:string:="z"%string.
+
+Inductive com : Type :=
+  | CSkip 
+  | CAss (x : string) (a : exp)
+  | CSeq (c1 c2 : com)
+  | CIf (a: exp) (c1 c2 : com)
+  | CWhile (a: exp) (c: com).
+
+Notation "'skip'"  :=
+         CSkip (in custom com at level 0) : com_scope.
+Notation "x := y"  :=
+         (CAss x y)
+            (in custom com at level 0, x constr at level 0,
+             y at level 85, no associativity) : com_scope.
+Notation "x ; y" :=
+         (CSeq x y)
+           (in custom com at level 90, right associativity) : com_scope.
+Notation "'if' x 'then' y 'else' z 'end'" :=
+         (CIf x y z)
+           (in custom com at level 89, x at level 99,
+            y at level 99, z at level 99) : com_scope.
+Notation "'while' x 'do' y 'end'" :=
+         (CWhile x y)
+   (in custom com at level 89, x at level 99, y at level 99) : com_scope.
+
+
+Fixpoint eval (a : exp) (s: state): exn nat :=
+  match a with
+  | ANum n       => Result n
+  | AId x        => Result (s x)  
+  | <{a1 + a2}>  => let n1:= (eval a1 s) in let n2:= (eval a2 s) in 
+                                match n1 with 
+                                  | Fail s    => Fail s
+                                  | Result m1 => match n2 with 
+                                        | Fail s => Fail s
+                                        | Result m2 => Result (m1 + m2) end end 
+  | <{a1 / a2}>  => let n1:= (eval a1 s) in let n2:= (eval a2 s) in 
+                                match n1 with 
+                                  | Fail s    => Fail s
+                                  | Result m1 => match n2 with 
+                                        | Fail s => Fail s
+                                        | Result m2 => match m2 with 
+                                                 | 0 => Fail "Division by zero!"
+                                                 | _ => Result (m1/m2) end end end 
+  | <{a1 == a2}> => let n1:= (eval a1 s) in let n2:= (eval a2 s) in 
+                                match n1 with 
+                                  | Fail s    => Fail s
+                                  | Result m1 => match n2 with 
+                                        | Fail s => Fail s
+                                        | Result m2 => match (beq_nat m1 m2) with 
+                                                        | true     => Result 0
+                                                        | false    => Result 1
+                                                                          end end end end .
+
+Example ex:exp := <{X+Y/Z+1}>.
+Compute  (eval ex (newarray 1)). 
+Compute  (eval ex empty_st). 
+
+Definition assign (x:string) (n:nat)(s: state):state := state_update s x n. 
+  
+Fixpoint exec (c: com)(fuel: nat): (state -> exn(unit * state)) :=
+match fuel with 
+| 0       => fun s=> Fail "Gas finished before end of program! Try executing with more gas."
+| S fuel' => match c with 
+        | <{ skip }>    => fun s => Result (tt, s)
+        | <{ x := a }>  => fun s => let m:=(eval a s) in match m with 
+                                                | Result n => Result (tt, state_update s x n)
+                                                | Fail str => Fail str end 
+        | <{c1; c2}>    => fun s => let o:= (exec c1 fuel') in match (o s) with 
+                                                | Fail str => Fail str
+                                                | Result (a, s') => 
+                                                    let o':= (exec c2 fuel') in (o' s') end 
+        | <{if a then c1 else c2 end}> => fun s => let m:=(eval a s) in match m with
+                                                | Fail str => Fail str 
+                                                | Result n => match n with 
+                                                          | 0 => (exec c1 fuel') s
+                                                          | _ => (exec c2 fuel') s end end 
+        |<{while b do c1 end}> => fun s => let m:=(eval b s) in match m with
+                                                | Fail str => Fail str
+                                                | Result b1 => match b1 with 
+                                                        | S _ => Result (tt, s)
+                                                        | 0   => match ((exec c1 fuel') s) with 
+                                                               | Result (a, s') => (exec c fuel') s'
+                                                               | Fail str => Fail str end end end 
+end end .
+                                                          
+Definition fact_in_coq : com :=
+  <{ Z := X;
+     Y := 1;
+     while X do
+       if Y == 5 then 
+         X:=1; X:=X/Z
+       else
+         Y := Y+1
+       end
+      end
+     }>.
+
+Definition eval_on_exn_state(es: exn (unit*state))(s: string): exn  nat:=
+match es with 
+| Fail str => Fail str 
+| Result (a, st) => Result (st s) end. 
+
+
+
+Compute  eval_on_exn_state((exec fact_in_coq 20) empty_st) X.
+   
+   
+ 
